dpe implementation complete, but uses an abstract hashtable interface and abstract DICE invocations.

share/steel/examples/pulse/dice/common/DPEPseudo.fst
@@ -15,41 +15,64 @@ open Array
 open HashTable
 
 friend Pulse.Steel.Wrapper
+#set-options "--print_implicits --print_universes"
+
+
+(* ----------- TYPES ----------- *)
 
 noeq
 type context_t = 
   | Engine_context  : uds:A.array U8.t -> 
                       context_t
-  | L0_context      : cdi:A.larray U8.t 32 -> 
+  | L0_context      : cdi:A.array U8.t -> 
                       context_t
   | L1_context      : aliasKey_priv:A.larray U8.t 32 ->
                       cert_aliasKey:A.array U8.t ->
                       csr_deviceID:A.array U8.t ->
                       context_t
 
+assume val destroy_ctxt (_:context_t) : unit
+
+// TODO: add remaining engine record fields
+noeq
+type engine_record_t = {
+  uds: A.array U8.t;
+  l0_image: A.array U8.t;
+}
+let mk_engine_record uds l0_image = {uds; l0_image}
+
+// TODO: add remaining engine record fields
+noeq
+type l0_record_t = {
+  cdi: A.array U8.t;
+  fwid: A.array U8.t;
+}
+let mk_l0_record cdi fwid = {cdi; fwid}
+
+
 (* ----------- GLOBAL STATE ----------- *)
 
 assume val dpe_hashf : nat -> nat
 assume val sht_len : pos
 assume val cht_len : pos
-let cht_sig = mk_ht_sig cht_len nat context_t dpe_hashf 
-let sht_sig = mk_ht_sig sht_len nat (ht_ref_t cht_sig) dpe_hashf 
+let cht_sig : ht_sig = mk_ht_sig cht_len nat context_t dpe_hashf 
+let sht_sig : ht_sig = mk_ht_sig sht_len nat (ht_ref_t cht_sig) dpe_hashf 
 
 // A table whose permission is stored in the lock 
 
 ```pulse
-fn alloc_ht (l:pos)
+fn alloc_ht (#s:ht_sig)
   requires emp
-  returns _:ht_ref_t
+  returns _:ht_ref_t s
   ensures emp
 {
-  let ht = new_table l;
-  let ht_ref = W.alloc #ht_t ht;
+  let ht = new_table #s;
+  let ht_ref = W.alloc #(ht_t s) ht;
   let lk = W.new_lock (exists_ (fun _ht -> R.pts_to ht_ref full_perm _ht));
-  ((| ht_ref, lk |) <: ht_ref_t)
+  ((| ht_ref, lk |) <: ht_ref_t s)
 }
 ```
-let sht_ref : ht_ref_t = alloc_ht sht_len ()
+let sht_ref : ht_ref_t sht_sig = alloc_ht #sht_sig ()
 
 // A number that tracks the next session ID
 
@@ -66,6 +89,7 @@ fn alloc_sid (_:unit)
 ```
 let sid_ref : sid_ref_t = alloc_sid () ()
 
+
 (* ----------- IMPLEMENTATION ----------- *)
 
 (*
@@ -79,7 +103,7 @@ fn open_session (_:unit)
   requires emp
   ensures emp
 {
-  let cht_ref = alloc_ht cht_len;
+  let cht_ref = alloc_ht #cht_sig;
 
   let l_sid = dsnd sid_ref;
   let l_sht = dsnd sht_ref;
@@ -164,54 +188,100 @@ fn initialize_context (sid:nat) (seed:A.array U8.t)
 }
 ```
 
-(*
-
-
-// DeriveChild: Part of DPE API 
-// Execute the DICE layer associated with the current context and produce a 
-// new context. Destroy the current context in the current session's context table 
-// and store the new context in the table. 
-fn DeriveChild (ctxt_hndl:A.array U32.t) (data:A.array U32.t) : A.array U32.t
-{
-  let cur_session = !session_id_ctr;
-  let session_tbl = acquire session_tbl_lock;
-  let ctxt_tbl_lock = get session_tbl cur_session;
-  let ctxt_tbl = acquire ctxt_tbl_lock;
-
-  let ctxt = get ctxt_tbl ctxt_hndl;
-  let new_hndl = (PRNG);
-  let new_ctxt: context_t = match ctxt
-  | Engine_context -> (
-      let engine_record = init_engine ctxt.uds data;
-      let cdi = engine_main engine_record;
-      L0_context cdi
-    )
-  | L0_context -> (
-      let l0_record = init_l0 ctxt.cdi data;
-      let (aliasKey_priv, cert_aliasKey, csr_deviceID) = l0_main l0_record;
-      L1_context aliasKey_priv cert_aliasKey csr_deviceID
-    )
-  | _ -> Error;
-
-  destroy ctxt_tbl ctxt_hndl;
-  store ctxt_tbl new_hndl new_ctxt;
-  new_hndl
-}
-
-
-// init_engine: Internal to DPE
-// Build the record of DICE Engine state given the uds and l0 image
-fn init_engine (uds:A.array U8.t) (l0_image:A.array U32.t) : engine_record_t
-{
-  ...
-}
-
-
-// init_l0: Internal to DPE
-// Build the record of DICE L0 state given the cdi and fwid
-fn init_l0 (cdi:A.larray U8.t 32) (fwid:A.array U32.t) : l0_record_t
-{
-  ...
-}
-
+(* call into DICE implementation *)
+assume val engine_main (_:engine_record_t) : c:context_t{L0_context? c}
+(* 
+  init_engine: Internal to DPE
+  Build the record of DICE Engine state given the uds and l0 image
 *)
+```pulse
+fn init_engine (ctxt:(c:context_t{Engine_context? c})) (data:A.array U8.t)
+  requires emp
+  returns _:engine_record_t
+  ensures emp
+{
+  admit();
+  // TODO: initialize remaining fields
+  // mk_engine_record ctxt.uds data
+}
+```
+
+(* call into DICE implementation *)
+assume val l0_main (_:l0_record_t) : c:context_t{L1_context? c}
+(*
+  init_l0: Internal to DPE
+  Build the record of DICE L0 state given the cdi and fwid
+*)
+```pulse
+fn init_l0 (ctxt:(c:context_t{L0_context? c})) (data:A.array U8.t)
+  requires emp
+  returns _:l0_record_t
+  ensures emp
+{
+  admit();
+  // TODO: initialize remaining fields
+  // mk_l0_record ctxt.cdi data
+}
+```
+
+(*
+  DeriveChild: Part of DPE API 
+  Execute the DICE layer associated with the current context and produce a 
+  new context. Destroy the current context in the current session's context table 
+  and store the new context in the table.
+  NOTE: Returns 0 if called when ctxt has type L1_context (bad invocation)
+*)
+```pulse
+fn derive_child (sid:nat) (ctxt_hndl:nat) (data:A.array U8.t)
+  requires emp
+  returns _:nat
+  ensures emp
+{
+  let new_ctxt_hndl = prng ();
+
+  let l_sht = dsnd sht_ref;
+  W.acquire #(exists_ (fun n -> R.pts_to (dfst sht_ref) full_perm n)) l_sht;
+  let sht = !(dfst sht_ref);
+
+  let cht_ref = get sht sid;
+
+  let l_cht = dsnd cht_ref;
+  W.acquire #(exists_ (fun n -> R.pts_to (dfst cht_ref) full_perm n)) l_cht;
+  let cht = !(dfst cht_ref);
+
+  let cur_ctxt = get cht ctxt_hndl;
+  let a = Engine_context? cur_ctxt;
+  let b = L0_context? cur_ctxt;
+  if a {
+    let engine_rec = init_engine cur_ctxt data;
+    let new_ctxt = engine_main engine_rec;
+    
+    destroy_ctxt cur_ctxt;
+    delete cht ctxt_hndl;
+    store cht new_ctxt_hndl new_ctxt;
+
+    W.release #(exists_ (fun n -> R.pts_to (dfst cht_ref) full_perm n)) l_cht;
+    W.release #(exists_ (fun n -> R.pts_to (dfst sht_ref) full_perm n)) l_sht;
+
+    new_ctxt_hndl
+  } else {
+    if b {
+      let l0_rec = init_l0 cur_ctxt data;
+      let new_ctxt = l0_main l0_rec;
+      
+      destroy_ctxt cur_ctxt;
+      delete cht ctxt_hndl;
+      store cht new_ctxt_hndl new_ctxt;
+
+      W.release #(exists_ (fun n -> R.pts_to (dfst cht_ref) full_perm n)) l_cht;
+      W.release #(exists_ (fun n -> R.pts_to (dfst sht_ref) full_perm n)) l_sht;
+
+      new_ctxt_hndl
+    } else {
+      W.release #(exists_ (fun n -> R.pts_to (dfst cht_ref) full_perm n)) l_cht;
+      W.release #(exists_ (fun n -> R.pts_to (dfst sht_ref) full_perm n)) l_sht;
+      0
+    };
+  };
+}
+```
